src/Init/Data/Iterators/Lemmas/Combinators/Monadic/FlatMap.lean
@@ -32,7 +32,7 @@ theorem IterM.step_flattenAfter {α α₂ β : Type w} {m : Type w → Type w'} 
   cases it₂
   all_goals
   · apply bind_congr; intro step
-    cases step.inflate using PlausibleIterStep.casesOn <;> simp [IterM.flattenAfter, IterM.mk]
+    cases step.inflate using PlausibleIterStep.casesOn <;> simp [IterM.flattenAfter]
 
 namespace Iterators.Types
 
